examples/low-level/array.fst
@@ -1,20 +1,37 @@
 (*--build-config
     options:--admit_fsi Set --z3timeout 10;
     variables:LIB=../../lib;
-    other-files:$LIB/ext.fst $LIB/set.fsi $LIB/heap.fst $LIB/st.fst $LIB/list.fst  stack.fst listset.fst st3.fst $LIB/constr.fst word.fst mvector.fsi
+    other-files:$LIB/ext.fst $LIB/set.fsi $LIB/heap.fst $LIB/st.fst $LIB/list.fst  stack.fst listset.fst st3.fst $LIB/constr.fst word.fst mvector.fsi mvector.fst array.fsi
   --*)
 
 (*rename mvector to vector. The word array is used for memory-stored vectors *)
-module MVector
+module Array
 open StructuredMem
 open MachineWord
 open Heap
 open Stack
 open Set
+open MVector
 
-let readIndex 'a #n r index =
-  let rv = (memread r) in (atIndex rv index)
+type array : Type -> Type =
+ | MkArr : #a:Type -> len:nat -> ref:(ref (vector a len)) -> array a
 
-let updIndex 'a #n r index newV =
-  let rv = (memread r) in
-  memwrite r (updateIndex rv index newV)
+(*Can we reinclude the types here, even when they are included in .fsi?
+  F* does not complain, even if we change the types*)
+ (*val length : #a:Type -> (array a) -> Tot string
+ let length v = "cat"*)
+
+
+(*val length : #a:Type -> (array a) -> Tot nat*)
+let length v = MkArr.len v
+
+val asRef : #a:Type  -> va:(array a) -> GTot (ref (vector a (length va)))
+let asRef va = MkArr.ref va
+
+
+let readIndex 'a r index =
+  let rv = (memread (MkArr.ref r)) in (atIndex rv index)
+
+let writeIndex 'a r index newV =
+  let rv = (memread (MkArr.ref r) ) in
+  memwrite (MkArr.ref r) (updateIndex rv index newV)
